\begin{description}
\item[Problem] Prove that
$$1^2 + 2^2 + \ldots + n^2 = \dfrac{n(n+1)(2n+1)}{6}$$
for $n \in \mathbb{N}$.

\item[Solution] For $n = 1$,
\begin{equation*}\begin{aligned}
1^2 &= \dfrac{1(1 + 1)(2 \cdot 1 + 1)}{6} \\
1   &= 1
\end{aligned}\end{equation*}

Given that $1^2 + 2^2 + \ldots + n^2 = \dfrac{n(n+1)(2n+1)}{6}$, for $n' = n +
1$ we have that
\begin{equation*}\begin{aligned}
1^2 + 2^2 + \ldots + n^2 + n'^2 &= \dfrac{n'(n'+1)(2n'+1)}{6} \\
(1^2 + 2^2 + \ldots + n^2) + (n+1)^2 &= \dfrac{(n+1)(n+2)(2n+3)}{6} \\
(1^2 + 2^2 + \ldots + n^2) + (n+1)^2 &= \dfrac{(n+1)(n+2)(2n+3)}{6} \\
\dfrac{n(n+1)(2n+1)}{6} + (n+1)^2 &= \dfrac{(n+1)(n+2)(2n+3)}{6} \\
(n+1)^2 &= \dfrac{(n+1)(n+2)(2n+3)}{6} - \dfrac{n(n+1)(2n+1)}{6} \\
(n+1)^2 &= \dfrac{(n+1)\left((n+2)(2n+3) - n(2n+1)\right)}{6} \\
(n+1)^2 &= \dfrac{(n+1)\left(6n + 6\right)}{6} \\
(n+1)^2 &= (n+1)^2
\end{aligned}\end{equation*}

\end{description}
