\begin{description}
\item[Problem] Prove that
$$1^3 + 2^3 + \cdots + n^3 = \dfrac {n^2 (n+1)^2} 4$$
for $n \in \mathbb{N}$.

\item[Proof] For $n = 1$,
\begin{equation*}\begin{aligned}
1^3 &= \dfrac{1^2 (1 + 1)^2}{4} \\
1   &= 1
\end{aligned}\end{equation*}

Given that $1^3 + 2^3 + \ldots + n^3 = \dfrac{n^2(n+1)^2}{4}$, for $n' = n + 1$
we have that
\begin{equation*}\begin{aligned}
1^3 + 2^3 + \cdots + n^3 + n'^3 &= \dfrac{n'^2 (n' + 1)^2}{4} \\
(1^3 + 2^3 + \cdots + n^3) + (n+1)^3 &= \dfrac{(n+1)^2 (n+2)^2} 4 \\
\dfrac{n^2(n+1)^2}{4} + (n+1)^3 &= \dfrac{(n+1)^2 (n+2)^2} 4 \\
(n+1)^3 &= \dfrac{(n+1)^2 (n+2)^2} 4 - \dfrac{n^2(n+1)^2}{4} \\
(n+1)^3 &= \dfrac{(n+1)^2 \left((n+2)^2 - n^2\right)} 4 \\
(n+1)^3 &= \dfrac{(n+1)^2 \left(4n + 4\right)} 4 \\
(n+1)^3 &= (n+1)^3 \\
\end{aligned}\end{equation*}

\end{description}

