\begin{description}
\item[Problem] Prove that
$$x + 4x + 7x + \cdots + (3n - 2)x = \dfrac{n(3n-1)x}{2}$$
for $n \in \mathbb{N}$.

\item[Proof] For $n = 1$,
\begin{equation*}\begin{aligned}
x &= \dfrac{1(3 \cdot 1 - 1)x}{2} \\
x &= x
\end{aligned}\end{equation*}

For $n' = n + 1$, given that $x + 4x + 7x + \cdots + (3n - 2)x =
\dfrac{n(3n-1)x}{2}$, we have
\begin{equation*}\begin{aligned}
x + 4x + 7x + \cdots + (3n - 2)x + (3n' - 2)x &= \dfrac{n'(3n'-1)x}{2} \\
(x + 4x + 7x + \cdots + (3n - 2)x) + (3n+1)x &= \dfrac{(n+1)(3n+2)x}{2} \\
\dfrac{n(3n-1)x}{2} + (3n + 1)x &= \dfrac{(n+1)(3n+2)x}{2} \\
(3n + 1)x &= \dfrac{(n+1)(3n+2)x}{2} - \dfrac{n(3n-1)x}{2} \\
(3n + 1)x &= \dfrac{\left((n+1)(3n+2) - n(3n-1)\right)x}{2} \\
(3n + 1)x &= \dfrac{\left(6n + 2\right)x}{2} \\
(3n + 1)x &= (3n + 1)x \\
\end{aligned}\end{equation*}

\end{description}
