\begin{description}
\item[Problem] Prove the Leibniz rules for $f^{(n)} (x)$, where $f^{(x)}$ is
the $n$th derivative of $f$; that is, show that
$$(fg)^{(n)}(x) = \sum\limits_{k = 0}^n {n \choose k} f^{(k)}(x)g^{(n-k)}(x).$$

\item[Proof] For $n = 1$,
\begin{align*}
(fg)'(x) &= \sum\limits_{k = 0}^1 {1 \choose k} f^{(k)}(x)g^{(1-k)}(x) \\
(fg)'(x) &= f(x)g'(x) + f'(x)g(x)
\end{align*}

As the induction hypothesis, we'll assume that the statement is correct for
$n$th derivative of product of any two functions. Then, for $n' = n + 1$,

\begin{align*}
(fg)^{(n')}(x) &= \sum\limits_{k = 0}^{n'} {n' \choose k}
f^{(k)}(x)g^{(n'-k)}(x) \\
(fg)^{(n+1)}(x) &= \sum\limits_{k = 0}^{n+1} {n+1 \choose k}
f^{(k)}(x)g^{(n+1-k)}(x) \\
\left((fg)^{(n)}\right)'(x) &=
\sum\limits_{k = 0}^{n+1} \left({n \choose k} + {n \choose k - 1}\right)
f^{(k)}(x)g^{(n+1-k)}(x) \\
\left((fg)^{(n)}\right)'(x) &=
\sum\limits_{k = 0}^{n+1} {n \choose k} f^{(k)}(x)g^{(n+1-k)}(x) +
\sum\limits_{k = 0}^{n+1} {n \choose k - 1} f^{(k)}(x)g^{(n+1-k)}(x) \\
\left((fg)^{(n)}\right)'(x) &=
\sum\limits_{k = 0}^{n} {n \choose k} f^{(k)}(x)g^{(n+1-k)}(x) +
\sum\limits_{k = 1}^{n+1} {n \choose k - 1} f^{(k)}(x)g^{(n+1-k)}(x) \\
\left((fg)^{(n)}\right)'(x) &=
\sum\limits_{k = 0}^{n} {n \choose k} f^{(k)}(x)g^{(n+1-k)}(x) +
\sum\limits_{k = 0}^{n} {n \choose k} f^{(k + 1)}(x)g^{(n-k)}(x) \\
\left((fg)^{(n)}\right)'(x) &=
\sum\limits_{k = 0}^{n} {n \choose k} f^{(k)}(x)(g')^{(n-k)}(x) +
\sum\limits_{k = 0}^{n} {n \choose k} (f')^{(k)}(x)g^{(n-k)}(x) \\
\left((fg)^{(n)}\right)'(x) &= (f(g'))^{(n)}(x) + ((f')g)^{(n)}(x) \\
((fg)')^{(n)}(x) &= \left(f(x)g'(x) + f'(x)g(x)\right)^{(n)} \\
((fg)')^{(n)}(x) &= ((fg)')^{(n)}(x)
\end{align*}

\end{description}
