\begin{description}
\item[Problem]
Prove $A \cap (B \cup C) = (A \cap B) \cup (A \cap C)$.

\item[Proof]

It suffices to observe by properties of logical relations that
\begin{equation*}
\begin{aligned}
A \cap (B \cup C) &= \left\{ x : x \in A\ \text{and}\ (x \in B\ \text{or}\ x
                       \in C) \right\}\\
                  &= \left\{ x : (x \in A\ \text{and}\ x \in B)\ \text{or}\ (x
                       \in A\ \text{and}\ x \in C) \right\}\\
                  &= \left\{ x : x \in A\ \text{and}\ x \in B\right\} \cup
                       \left\{ x : x \in A\ \text{and}\ x \in C \right\}\\
                  &= (A \cap B) \cup (A \cap C)
\end{aligned}
\end{equation*}

\end{description}
