\begin{description}
\item[Problem]
Prove $(A \cup B) \times C = (A \times C) \cup (B \times C)$.

\item[Proof]~\\
\begin{equation*}
\begin{aligned}
(A \cup B) \times C &= \left\{ (x, c) : (x \in A\ \text{or}\ x \in B)\ 
\text{and}\ c \in C\right\} \\
&= \left\{ (x, c) : x \in A\ \text{and}\ c \in C\ \text{or}\ x \in B\ 
\text{and}\ c \in C\right\} \\
&= \left\{ (x, c) : x \in A\ \text{and}\ c \in C \right\} \cup
\left\{ (x, c) : x \in B\ \text{and}\ c \in C \right\} \\
&= (A \times C) \cup (B \times C)
\end{aligned}
\end{equation*}

\end{description}
