\begin{description}
\item[Problem]
Prove $A \setminus (B \cup C) = (A \setminus B) \cap (A \setminus C)$.

\item[Proof]~\\
\begin{equation*}
\begin{aligned}
A \setminus (B \cup C)
                 &= \left\{ x : x \in A\ \text{and}\ x \not \in (B \cup C)
                    \right\} \\
                 &= \left\{ x : x \in A\ \text{and}\ x \not \in B\ 
                    \text{and}\ x \not \in C\right\} \\
                 &= \left\{ x : (x \in A\ \text{and}\ x \not \in B)\ 
                    \text{and}\ (x \in A\ \text{and}\ x \not \in C)\right\} \\
                 &= \left\{ x : (x \in A\ \text{and}\ x \not \in B)\right\}
                    \cap
                    \left\{ x : (x \in A\ \text{and}\ x \not \in C)\right\} \\
                 &= (A \setminus B) \cap (A \setminus C)
\end{aligned}
\end{equation*}

\end{description}

