\begin{description}
\item[Problem]
Prove $A \cap (B \setminus C) = (A \cap B) \setminus (A \cap C)$.

\item[Proof]~\\
\begin{equation*}
\begin{aligned}
A \cap (B \setminus C)
        &= \left\{ x : x \in A \land x \in (B \setminus C)\right\} \\
        &= \left\{ x : x \in A \land x \in B \land x \not \in C\right\} \\
        &= \left\{ x : (x \in A \land x \in B \land x \not \in C) \lor
           \mathbf{false}\right\} \\
        &= \left\{ x : (x \in A \land x \in B \land x \not \in C) \lor
           (x \in A \land x \in B \land x \not \in A)\right\} \\
        &= \left\{ x : x \in A \land x \in B \land (x \not \in C \lor x \not
           \in A) \right\} \\
        &= \left\{ x : (x \in A \land x \in B) \land \neg (x \in C \land x \in
           A) \right\} \\
        &= \left\{ x : x \in A \land x \in B \right\} \setminus 
           \left\{ x : x \in C \land x \in A \right\} \\
        &= (A \cap B) \setminus (A \cap C)
\end{aligned}
\end{equation*}

\end{description}
