\begin{description}
\item[Problem]
Prove $(A \setminus B) \cup (B \setminus A) = (A \cup B) \setminus (A \cap B)$.

\item[Proof]~\\
\begin{equation*}
\begin{aligned}
(A \setminus B) \cup (B \setminus A)
        &= \left\{ x : x \in (A \setminus B) \lor x \in (B \setminus A)
           \right\} \\
        &= \left\{ x : x \in A \land x \not \in B \lor x \in B \land x \not
           \in A\right\} \\
        &\begin{aligned}
         = \{ x : &(x \in A \land x \not \in B) \lor
                  (x \in B \land x \not \in A) \lor \\
                  &(x \in A \land x \not \in A) \lor
                  (x \in B \land x \not \in B)\}
        \end{aligned}\\
        &= \left\{ x : (x \in A \land (x \not \in A \lor x \not \in B)) \lor
                       (x \in B \land (x \not \in A \lor x \not \in B))
           \right\} \\
        &= \left\{ x : (x \in A \lor x \in B) \land (x \not \in A \lor x
           \not \in B)\right\} \\
        &= \left\{ x : (x \in A \lor x \in B) \land \neg (x \in A \land x
           \in B)\right\} \\
        &= \left\{ x : x \in A \lor  x \in B\right\} \setminus
           \left\{ x : x \in A \land x \in B\right\} \\
        &= (A \cup B) \setminus (A \cap B)
\end{aligned}
\end{equation*}
\end{description}
