\begin{description}
\item[Problem] Let $f : A \rightarrow B$ and $g : B \rightarrow C$ be
invertible mappings; that is, mappings such that $f^{-1}$ and $g^{-1}$ exist.
Show that $(g \circ f)^{-1} = f^{-1} \circ g^{-1}$.
\item[Proof] Let $c \in C$. Let $b$ be its pre-image in $B$, and $a$ the
pre-image of $b$ in $A$. Then $b = g^{-1} (c)$, $a = f^{-1} (b)$. By definition
of function composition, it can be written as $a = \left(f^{-1} \circ
g^{-1}\right)(c)$. Conversely, $b = f(a)$, $c = f(b)$, and $c = (g
\circ f)(a)$. By definition of function inverse, $(g \circ f)^{-1} =
f^{-1} \circ g^{-1}$.
\end{description}
