\begin{description}
\item[Problem] Prove the relation defined on $\mathbb{R}^2$ by $(x_1, y_1)
\sim (x_2, y_2)$ if $x_1^2 + y_1^2 = x_2^2 + y_2^2$ is an equivalence
relation.
\item[Proof] The equivalence relation must satisfy the following properties:
\begin{description}
        \item[Symmetry] $(x, y) \sim (x, y)$ since $x^2 + y^2 = x^2 + y^2$.
        \item[Reflexivity] $(x_1, y_1) \sim (x_2, y_2) \iff (x_2, y_2) \sim
                (x_1, y_1)$ since $x_2^2 + y_2^2 = x_1^2 + y_1^2$ follows from
                $x_1^2 + y_1^2 = x_2^2 + y_2^2$.
        \item[Transitivity] $(x_1, y_1) \sim (x_2, y_2), (x_2, y_2) \sim
                (x_3, y_3) \rightarrow (x_1, y_1) \sim (x_3, y_3)$ is also
                evident: $x_1^2 + y_1^2 = x_2^2 + y_2^2 = x_3^2 + y_3^2$.
\end{description}
\end{description}
